WIP on using a generic version of conversion + typing

theories/Untyped.v
@@ -2,7 +2,7 @@ From MetaCoq.PCUIC Require Import PCUICAst PCUICAstUtils PCUICNormal.
 From LogRel Require Import Automation.
 
 Definition U := (tSort Universe.type0).
-Definition eta_expand (f : term) := tApp (lift0 1 f) (tRel 0).
+Notation "'eta_expand' f" := (tApp (lift0 1 f) (tRel 0)) (at level 40, only parsing).
 
 #[global] Hint Transparent U : mltt.
 
