theories/Automation.v
@@ -1,6 +1,0 @@
-
-Create HintDb mltt.
-#[global] Hint Constants Opaque : mltt.
-#[global] Hint Variables Transparent : mltt.
-
-Ltac mltt := eauto with mltt.
