theories/DeclarativeTyping.v
@@ -177,95 +177,6 @@ Inductive typeRed (Γ : context) : term -> term -> Type :=
 
 where "[ Γ |- A ⇒ B ]" := (typeRed Γ A B).
 
-Inductive termRedClosure (Γ : context) : term -> term -> term -> Type :=
-    | termRedId {t A} :
-        [ Γ |- t : A ] ->
-        [ Γ |- t ⇒* t : A ]
-    | termRedSucc {A t t' u} :
-        [ Γ |- t ⇒ t' : A ] ->
-        [ Γ |- t' ⇒* u : A ] ->
-        [ Γ |- t ⇒* u : A ]
-
-where "[ Γ |- t ⇒* t' : A ]" := (termRedClosure Γ t t' A).
-
-Inductive typeRedClosure (Γ : context) : term -> term -> Type :=
-| typeRedId {A} :
-    [ Γ |- A  ] ->
-    [ Γ |- A ⇒* A]
-| typeRedSucc {A A' B} :
-    [ Γ |- A ⇒ A' ] ->
-    [ Γ |- A' ⇒* B ] ->
-    [ Γ |- A ⇒* B ]
-
-where "[ Γ |- A ⇒* B ]" := (typeRedClosure Γ A B).
-
-(* Record termRedStrict (Γ : context) (t u A : term) {t'} : Type :=
-  {
-    termRedStrictOneRed : [ Γ |- t ⇒ t' : A ] ;
-    termRedStrictRed : [Γ |- t' ⇒* u : A]
-  }.
-
-Notation  "[ Γ |- t ⇒⁺ u : A ]" := (termRedStrict Γ t u A).
-
-Record typeRedStrict (Γ : context) (A B : term) {A'} : Type :=
-  {
-    typeRedStrictOneRed : [ Γ |- A ⇒ A'] ;
-    typeRedStrictRed : [Γ |- A' ⇒* B]
-  }.
-
-Notation "[ Γ |- t ⇒⁺ u : A ]" := (termRedStrict Γ t u A). *)
-
-Record typeRedWHNF (Γ : context) (A B : term) : Type :=
-  {
-    typeRedWHNFRed :> [ Γ |- A ⇒* B ] ;
-    typeRedWHNFWHNF :> whnf Γ B
-  }.
-
-Notation "[ Γ |- A ↘ B ]" := (typeRedWHNF Γ A B).
-
-
-Record termRedWHNF (Γ : context) (t u A : term) : Type :=
-  {
-    termRedWHNFRed :> [ Γ |- t ⇒* u : A ] ;
-    termRedWHNFWHNF :> whnf Γ u
-  }.
-
-Notation "[ Γ |- t ↘ u : A ]" := (termRedWHNF Γ t u A).
-
-Record typeEqWF (Γ : context) (A B : term) : Type :=
-  { 
-    typeEqWFLeft : [Γ |- A] ;
-    typeEqWFRight : [Γ |- B] ;
-    typeEqWFEq :> [Γ |- A ≅ B]
-  }.
-
-Notation "[ Γ |- A :≅: B ]" := (typeEqWF Γ A B).
-
-Record termEqWF (Γ : context) (t u A : term) : Type :=
-  {
-    termEqWFLeft : [Γ |- t : A] ;
-    termEqWFRight : [Γ |- u : A] ;
-    termEqWFEq :> [Γ |- t ≅ u : A]
-  }.
-
-Notation "[ Γ |- t :≅: u : A ]" := (termEqWF Γ t u A).
-
-Record typeRedWF (Γ : context) (A B : term) : Type := {
-  typeRedWFLeft : [Γ |- A];
-  typeRedWFRight : [Γ |- B];
-  typeRedWFRed :> [Γ |- A ⇒* B]
-}.
-
-Notation "[ Γ |- A :⇒*: B ]" := (typeRedWF Γ A B).
-
-Record termRedWF (Γ : context) (t u A : term) : Type := {
-  termRedWFLeft : [Γ |- t : A];
-  termRedWFRight : [Γ |- u : A];
-  termRedWFRed :> [Γ |- t ⇒* u : A]
-}.
-
-Notation "[ Γ |- t :⇒*: u : A ]" := (termRedWF Γ t u A).
-
 #[global] Hint Constructors wfType wfContext wfTerm convType convTerm : mltt.
 #[global] Hint Constructors termRed typeRed termRedClosure typeRedClosure
   termRedWHNF typeRedWHNF termEqWF typeEqWF termRedWF typeRedWF : mltt.
@@ -280,3 +191,196 @@ Notation "[ Γ |- t :⇒*: u : A ]" := (termRedWF Γ t u A).
   termEqWFLeft termEqWFRight termEqWFEq typeEqWFLeft typeEqWFRight typeEqWFEq
   termRedWFLeft termRedWFRight termRedWFRed typeRedWFLeft typeRedWFRight
   typeRedWFRed : mltt.
+
+
+Section TypingWk.
+
+Variable foo : context_decl.
+
+Lemma nth_error_wk (Γ Δ : context) n decl (ρ : Δ ≤ Γ) :
+  nth_error Γ n = Some decl ->
+  {decl' & nth_error Δ (ρ n) = Some decl' ×
+    map_decl (rename (ρ ∘ rshiftk (S n))) decl = map_decl (rename (rshiftk (S (ρ n)))) decl'}.
+Proof.
+  intros Hdecl.
+  destruct ρ as [ρ wfρ] ; cbn.
+  induction wfρ in n, Hdecl |- *.
+  - exists decl.
+    split.
+    1: easy.
+    reflexivity.
+  - cbn.
+    edestruct IHwfρ as [decl' [? IH]].
+    1: eassumption.
+    eexists ; split.
+    1: eassumption.
+    now rewrite <- rename_compose, <- compose_map_decl, IH, compose_map_decl, rename_compose.
+  - destruct n as [ | n].
+    + cbn in *.
+      inversion Hdecl ; subst ; clear Hdecl.
+      eexists ; split.
+      1: reflexivity.
+      unfold map_decl ; cbn.
+      f_equal.
+      rewrite <- rename_inst, rename_compose.
+      apply rename_ext.
+      intros ?.
+      now rewrite Nat.sub_0_r.
+    + cbn in *.
+      edestruct IHwfρ as [decl' [? IH]].
+      1: eassumption.
+      eexists ; split.
+      1: now rewrite Nat.sub_0_r.
+      now rewrite <- rename_compose, <- compose_map_decl, IH, compose_map_decl, rename_compose, Nat.sub_0_r.
+  Qed.
+
+Let PCon (Γ : context) := True.
+Let PTy (Γ : context) (A : term) := forall Δ (ρ : Δ ≤ Γ), [|- Δ ] -> [Δ |- A.[ren ρ]].
+Let PTm (Γ : context) (t A : term) := forall Δ (ρ : Δ ≤ Γ), [|- Δ ] ->
+  [Δ |- t.[ren ρ] : A.[ren ρ]].
+Let PTyEq (Γ : context) (A B : term) := forall Δ (ρ : Δ ≤ Γ), [|- Δ ] ->
+  [Δ |- A.[ren ρ] ≅ B.[ren ρ]].
+Let PTmEq (Γ : context) (t u A : term) := forall Δ (ρ : Δ ≤ Γ), [|- Δ ] ->
+  [Δ |- t.[ren ρ] ≅ u.[ren ρ] : A.[ren ρ]].
+
+
+Theorem typing_wk : wfInductionType PCon PTy PTm PTyEq PTmEq.
+Proof.
+  apply wfInduction.
+  - red.
+    trivial.
+  - red. trivial.
+  - intros ? ? IH.
+    now econstructor.
+  - intros Γ na A B HA IHA HB IHB Δ ρ HΔ.
+    econstructor ; fold inst.
+    1: easy.
+    replace (B.[up 1 (ren ρ)]) with (B.[ren (wk_lift ρ)])
+      by now rewrite ren_shiftn.
+    unshelve eapply (IHB _ {| wk := wk_lift ρ ; well_wk := _ |} _).
+    all: now econstructor.
+  - intros * _ IHA ? * ?.
+    econstructor.
+    now eapply IHA.
+  - intros * _ IHΓ Hnth ? * ?.
+    unshelve eapply nth_error_wk in Hnth as [decl' [? edecl]] ; tea.
+    unfold ren at 1.
+    cbn.
+    eapply termMetaConv.
+    1: econstructor ; eassumption.
+    rewrite <- rename_inst, ! lift_rename, rename_compose, (map_decl_type _ decl'), (map_decl_type _ decl).
+    f_equal.
+    rewrite ! lift_renaming_0_rshift, <- edecl.
+    eapply map_decl_ext ; intros ; eapply rename_ext ; intros ?.
+    now rewrite lift_renaming_0_rshift.
+  - intros * _ IHA _ IHB ? ρ ?.
+    cbn.
+    econstructor.
+    1: now eapply IHA.
+    replace B.[_] with B.[ren (wk_lift ρ)] by now rewrite ren_shiftn.
+    unshelve eapply (IHB _ {| wk := wk_lift ρ ; well_wk := _ |} _).
+    1: now econstructor.
+    econstructor ; tea.
+    econstructor.
+    now eapply IHA.
+  - intros * _ IHA _ IHt ? ρ ?.
+    cbn.
+    econstructor.
+    1: now eapply IHA.
+    red in IHt.
+    replace t.[_] with t.[ren (wk_lift ρ)] by now rewrite ren_shiftn.
+    replace B.[_] with B.[ren (wk_lift ρ)] by now rewrite ren_shiftn.
+    unshelve eapply (IHt _ {| wk := wk_lift ρ ; well_wk := _ |} _).
+    1: now econstructor.
+    econstructor ; tea.
+    now eapply IHA.
+  - intros * _ IHf _ IHu ? ρ ?.
+    cbn.
+    rewrite subst10_inst.
+    replace B.[_] with B.[(up 1 (ren ρ))] by (now rewrite up_Up).
+    econstructor.
+    2: now eapply IHu.
+    now eapply IHf.
+  - intros * _ IHt _ IHAB ? ρ ?.
+    econstructor.
+    1: now eapply IHt.
+    now eapply IHAB.
+  - intros Γ ? ? A A' B B' _ IHA _ IHAA' _ IHBB' ? ρ ?.
+    cbn.
+    econstructor.
+    + now eapply IHA.
+    + now eapply IHAA'.
+    + replace B.[_] with B.[ren (wk_lift ρ)] by now rewrite ren_shiftn.
+      replace B'.[_] with B'.[ren (wk_lift ρ)] by now rewrite ren_shiftn.
+      unshelve eapply (IHBB' _ {| wk := wk_lift ρ ; well_wk := _ |} _).
+      1: now econstructor.
+      econstructor ; tea.
+      now eapply IHA.
+  - intros * _ IHA ? ρ ?.
+    eapply TypeRefl.
+    now eapply IHA.
+  - intros * _ IH ? ρ ?.
+    econstructor.
+    now eapply IH.
+  - intros * _ IHA _ IHB ? ρ ?.
+    eapply TypeTrans.
+    + now eapply IHA.
+    + now eapply IHB.
+  - intros * _ IH ? ρ ?.
+    eapply convUniv.
+    now eapply IH.
+  - intros Γ ? ? A A' B B' _ IHA _ IHAA' _ IHBB' ? ρ ?.
+    cbn.
+    econstructor.
+    + now eapply IHA.
+    + now eapply IHAA'.
+    + replace B.[_] with B.[ren (wk_lift ρ)] by now rewrite ren_shiftn.
+      replace B'.[_] with B'.[ren (wk_lift ρ)] by now rewrite ren_shiftn.
+      unshelve eapply (IHBB' _ {| wk := wk_lift ρ ; well_wk := _ |} _).
+      all: now econstructor.
+  - intros Γ ? u u' f f' A B _ IHf _ IHu ? ρ ?.
+    cbn.
+    rewrite subst10_inst.
+    replace B.[_] with B.[(up 1 (ren ρ))] by (now rewrite up_Up).
+    now econstructor.
+  - intros Γ ? u t A B _ IHA _ IHt _ IHu ? ρ ?.
+    cbn. 
+    rewrite ! subst10_inst.
+    replace t.[⇑ _] with t.[(up 1 (ren ρ))] by (now rewrite up_Up).
+    replace t.[_] with t.[ren (wk_lift ρ)] by (now rewrite ren_shiftn).
+    replace B.[_] with B.[ren (wk_lift ρ)] by (now rewrite <- up_Up, ren_shiftn).
+    econstructor.
+    1,3: easy.
+    unshelve eapply (IHt _ {| wk := wk_lift ρ ; well_wk := _ |} _).
+    all: now econstructor.
+  - intros Γ ? ? f f' A B _ IHA _ IHf _ IHg _ IHe ? ρ ?.
+    cbn.
+    econstructor.
+    1-3: easy.
+    unshelve epose proof (IHe _ {| wk := wk_lift ρ ; well_wk := _ |} _) as IHe'.
+    2: now econstructor.
+    1: now econstructor.
+    cbn in *.
+    unfold ren in IHe' at 3 5.
+    unfold eta_expand.
+    cbn in *.
+    rewrite ! lift0_inst, ! inst_assoc in IHe' |- *.
+    replace B.[_] with B.[ren (shiftn 1 ρ)] by (now rewrite ren_shiftn).
+    unshelve erewrite (inst_ext _ _ _ f), (inst_ext _ _ _ f').
+    5: eassumption.
+    all: rewrite <- Upn_ren.
+    all: change 1 with (0 + 1).
+    all: rewrite <- subst_shift_comm.
+    all: cbn.
+    all: now rewrite Upn_0.
+  - intros * _ IHt ? ρ ?.
+    now econstructor.
+  - intros * _ IHt ? ρ ?.
+    now econstructor.
+  - intros * _ IHt _ IHt' ? ρ ?.
+    now eapply TermTrans.
+  - intros * _ IHt _ IHA ? ρ ?.
+    now eapply TermConv.
+Qed.
+
+End TypingWk.
