theories/GenericTyping.v
@@ -1,0 +1,374 @@
+From Coq Require Import CRelationClasses.
+From MetaCoq.PCUIC Require Import PCUICAst PCUICAstUtils PCUICRenameConv PCUICSigmaCalculus PCUICInstConv.
+From LogRel Require Import Notations Untyped Weakening.
+
+(* The database used for generic typing *)
+Create HintDb gen_typing.
+#[global] Hint Constants Opaque : gen_typing.
+#[global] Hint Variables Transparent : gen_typing.
+
+Ltac gen_typing := typeclasses eauto 10 with gen_typing typeclass_instances.
+
+Class GenericTypingData (ta : tag) := {
+  wfc :> WfContext ta ;
+  wf_ty :> WfType ta ;
+  ty :> Typing ta ;
+  co_ty :> ConvType ta ;
+  co_tm :> ConvTerm ta ;
+  co_ne :> ConvNeu ta ;
+  red_ty :> OneRedType ta ;
+  red_tm :> OneRedTerm ta
+  }.
+
+Section RedDefinitions.
+
+  Open Scope untagged_scope.
+
+  Context {ta : tag}
+    `{wfc : !WfContext ta} `{wf_ty : !WfType ta} `{ty : !Typing ta}
+    `{co_ty : !ConvType ta} `{co_tm : !ConvTerm ta} `{co_ne : !ConvNeu ta}
+    `{red_ty : !OneRedType ta} `{red_tm : !OneRedTerm ta}.
+
+  Inductive TermRedClosure (Γ : context) : term -> term -> term -> Type :=
+      | term_red_id {t A} :
+          [ Γ |- t : A ] ->
+          [ Γ |- t ⇒* t : A ]
+      | term_red_succ {A t t' u} :
+          [ Γ |- t ⇒ t' : A ] ->
+          [ Γ |- t' ⇒* u : A ] ->
+          [ Γ |- t ⇒* u : A ]
+
+  where "[ Γ |- t ⇒* t' : A ]" := (TermRedClosure Γ t t' A).
+
+  Inductive TypeRedClosure (Γ : context) : term -> term -> Type :=
+  | type_red_id {A} :
+      [ Γ |- A ] ->
+      [ Γ |- A ⇒* A]
+  | type_red_succ {A A' B} :
+      [ Γ |- A ⇒ A' ] ->
+      [ Γ |- A' ⇒* B ] ->
+      [ Γ |- A ⇒* B ]
+
+  where "[ Γ |- A ⇒* B ]" := (TypeRedClosure Γ A B).
+
+  Record TypeRedWhnf (Γ : context) (A B : term) : Type :=
+    {
+      tyred_whnf_red :> [ Γ |- A ⇒* B ] ;
+      tyred_whnf_whnf :> whnf Γ B
+    }.
+
+  Record TermRedWhnf (Γ : context) (t u A : term) : Type :=
+    {
+      tmred_whnf_red :> [ Γ |- t ⇒* u : A ] ;
+      tmred_whnf_whnf :> whnf Γ u
+    }.
+
+  Record TypeConvWf (Γ : context) (A B : term) : Type :=
+    { 
+      tyc_wf_l : [Γ |- A] ;
+      tyc_wf_r : [Γ |- B] ;
+      tyc_wf_conv :> [Γ |- A ≅ B]
+    }.
+
+  Record TermConvWf (Γ : context) (t u A : term) : Type :=
+    {
+      tmc_wf_l : [Γ |- t : A] ;
+      tmc_wf_r : [Γ |- u : A] ;
+      tmc_wf_conv :> [Γ |- t ≅ u : A]
+    }.
+
+  Record TypeRedWf (Γ : context) (A B : term) : Type := {
+    tyr_wf_l : [Γ |- A];
+    tyr_wf_r : [Γ |- B];
+    tyr_wf_red :> [Γ |- A ⇒* B]
+  }.
+
+  Record TermRedWf (Γ : context) (t u A : term) : Type := {
+    tmr_wf_l : [Γ |- t : A];
+    tmr_wf_r : [Γ |- u : A];
+    tmr_wf_red :> [Γ |- t ⇒* u : A]
+  }.
+
+End RedDefinitions.
+
+Notation "[ Γ |- t ⇒* t' : A ]" := (TermRedClosure Γ t t' A) : untagged_scope.
+Notation "[ Γ |-[ ta  ] t ⇒* t' : A ]" := (TermRedClosure (ta := ta) Γ t t' A) : tagged_scope.
+Notation "[ Γ |- A ⇒* B ]" := (TypeRedClosure Γ A B) : untagged_scope.
+Notation "[ Γ |-[ ta  ] A ⇒* B ]" := (TypeRedClosure (ta := ta) Γ A B) : tagged_scope.
+Notation "[ Γ |- A ↘ B ]" := (TypeRedWhnf Γ A B) : untagged_scope.
+Notation "[ Γ |-[ ta  ] A ↘ B ]" := (TypeRedWhnf (ta := ta) Γ A B) : tagged_scope.
+Notation "[ Γ |- t ↘ u : A ]" := (TermRedWhnf Γ t u A) : untagged_scope.
+Notation "[ Γ |-[ ta  ] t ↘ u : A ]" := (TermRedWhnf (ta := ta) Γ t u A) : tagged_scope.
+Notation "[ Γ |- A :≅: B ]" := (TypeConvWf Γ A B) : untagged_scope.  
+Notation "[ Γ |-[ ta  ] A :≅: B ]" := (TypeConvWf (ta := ta) Γ A B) : tagged_scope.
+Notation "[ Γ |- t :≅: u : A ]" := (TermConvWf Γ t u A) : untagged_scope.
+Notation "[ Γ |-[ ta  ] t :≅: u : A ]" := (TermConvWf (ta := ta) Γ t u A) : tagged_scope.
+Notation "[ Γ |- A :⇒*: B ]" := (TypeRedWf Γ A B) : untagged_scope.
+Notation "[ Γ |-[ ta  ] A :⇒*: B ]" := (TypeRedWf (ta := ta) Γ A B) : tagged_scope.
+Notation "[ Γ |- t :⇒*: u : A ]" := (TermRedWf Γ t u A) : untagged_scope.
+Notation "[ Γ |-[ ta  ] t :⇒*: u : A ]" := (TermRedWf (ta := ta) Γ t u A) : tagged_scope.
+
+
+#[export] Hint Resolve
+  term_red_id term_red_succ type_red_id type_red_succ
+  Build_TypeRedWhnf Build_TermRedWhnf Build_TypeConvWf
+  Build_TermConvWf Build_TypeRedWf Build_TermRedWf
+  : gen_typing.
+
+#[export] Hint Extern 1 =>
+  match goal with
+    |  H : [ _ |- _ ↘ _ ]%untagged |- _ => destruct H
+    |  H : [ _ |- _ ↘ _ : _ ]%untagged |- _ => destruct H
+    |  H : [ _ |- _ :≅: _ ]%untagged |- _ => destruct H
+    |  H : [ _ |- _ :≅: _ : _]%untagged |- _ => destruct H
+    |  H : [ _ |- _ :⇒*: _ : _ ]%untagged |- _ => destruct H
+  end
+  : gen_typing.
+
+Section GenericTyping.
+
+  Open Scope untagged_scope.
+
+  Context {ta : tag}
+    `{wfc : !WfContext ta} `{wf_ty : !WfType ta} `{ty : !Typing ta}
+    `{co_ty : !ConvType ta} `{co_tm : !ConvTerm ta} `{co_ne : !ConvNeu ta}
+    `{red_ty : !OneRedType ta} `{red_tm : !OneRedTerm ta}.
+
+  Class WfContextProp :=
+  {
+    wfc_nil : [|- []] ;
+    wfc_cons {Γ na A} : [|- Γ] -> [Γ |- A] -> [|- Γ,,vass na A]
+  }.
+
+  Class WfTypeProp :=
+  {
+    wft_U {Γ} : 
+      [ |- Γ ] -> 
+      [ Γ |- U ] ;
+    wft_prod {Γ} {na : aname} {A B} : 
+      [ Γ |- A ] -> 
+      [Γ ,, (vass na A) |- B ] -> 
+      [ Γ |- tProd na A B ] ;
+    wft_term {Γ} {A} :
+      [ Γ |- A : U ] -> 
+      [ Γ |- A ] ;
+  }.
+
+  Class TypingProp :=
+  {
+    ty_var {Γ} {n decl} :
+      [   |- Γ ] ->
+      nth_error Γ n = Some decl ->
+      [ Γ |- tRel n : lift0 (S n) decl.(decl_type) ] ;
+    ty_prod {Γ} {na} {A B} :
+        [ Γ |- A : U] -> 
+        [Γ ,, (vass na A) |- B : U ] ->
+        [ Γ |- tProd na A B : U ] ;
+    ty_lam {Γ} {na} {A B t} :
+        [ Γ |- A ] ->        
+        [ Γ ,, vass na A |- t : B ] -> 
+        [ Γ |- tLambda na A t : tProd na A B] ;
+    ty_app {Γ} {na} {f a A B} :
+        [ Γ |- f : tProd na A B ] -> 
+        [ Γ |- a : A ] -> 
+        [ Γ |- tApp f a : B{0 := a} ] ;
+    ty_conv {Γ t A A'} : [Γ |- t : A] -> [Γ |- A ≅ A'] -> [Γ |- t : A'] ;
+  }.
+
+  Class ConvTypeProp :=
+  {
+    convty_term {Γ A B} : [Γ |- A ≅ B : U] -> [Γ |- A ≅ B] ;
+    convty_equiv {Γ} :> PER (fun A B => [Γ |- A ≅ B]) ;
+    convty_wk {Γ Δ A B} (ρ : Γ ≤ Δ) :
+      [Γ |- A ≅ B] -> [Δ |- A.[ren ρ] ≅ B.[ren ρ]] ;
+    convty_whexp {Γ A A' B B'} :
+      [Γ |- A ⇒* A'] -> [Γ |- B ⇒* B'] ->
+      [Γ |- A' ≅ B'] -> [Γ |- A ≅ B] ;
+    convty_uni {Γ} :
+      [Γ |- U ≅ U] ;
+    convty_prod {Γ na na' A A' B B'} :
+      eq_binder_annot na na' ->
+      [Γ |- A ≅ A'] -> [Γ,, vass na A |- B ≅ B'] ->
+      [Γ |- tProd na A B ≅ tProd na' A' B'] ;
+  }.
+
+  Class ConvTermProp :=
+  {
+    convtm_equiv {Γ A} :> PER (fun t u => [Γ |- t ≅ u : A]) ;
+    convtm_conv {Γ t u A A'} : [Γ |- t ≅ u : A] -> [Γ |- A ≅ A'] -> [Γ |- t ≅ u : A'] ;
+    convtm_wk {Γ Δ t u A} (ρ : Γ ≤ Δ) :
+      [Γ |- t ≅ u : A] -> [Δ |- t.[ren ρ] ≅ u.[ren ρ] : A.[ren ρ]] ;
+    convtm_whexp {Γ A A' t t' u u'} :
+      [Γ |- A ⇒* A'] -> [Γ |- t ⇒* t' : A'] -> [Γ |- u ⇒* u' : A'] ->
+      [Γ |- t' ≅ u' : A'] -> [Γ |- t ≅ u : A] ;
+    convtm_convneu {Γ n n' A} :
+      [Γ |- n ~ n' : A] -> [Γ |- n ≅ n' : A] ;
+    convtm_prod {Γ na na' A A' B B'} :
+      eq_binder_annot na na' ->
+      [Γ |- A ≅ A' : U] -> [Γ,, vass na A |- B ≅ B' : U] ->
+      [Γ |- tProd na A B ≅ tProd na' A' B' : U] ;
+    convtm_eta {Γ na f g A B} :
+      [ Γ |- A ] ->
+      [ Γ |- f : tProd na A B ] ->
+      [ Γ |- g : tProd na A B ] ->
+      [ Γ ,, vass na A |- eta_expand f ≅ eta_expand g : B ] ->
+      [ Γ |- f ≅ g : tProd na A B ] ;
+  }.
+
+  Class ConvNeuProp :=
+  {
+    convneu_equiv {Γ A} :> PER (fun t u => [Γ |- t ~ u : A]) ;
+    convneu_conv {Γ t u A A'} : [Γ |- t ~ u : A] -> [Γ |- A ≅ A'] -> [Γ |- t ~ u : A'] ;
+    convneu_wk {Γ Δ t u A} (ρ : Γ ≤ Δ) :
+      [Γ |- t ~ u : A] -> [Δ |- t.[ren ρ] ~ u.[ren ρ] : A.[ren ρ]] ;
+    convneu_var {Γ n A} :
+      [Γ |- tRel n : A] -> [Γ |- tRel n ~ tRel n : A] ;
+    convneu_app {Γ f g t u na A B} :
+        [ Γ |- f ~ g : tProd na A B ] ->
+        [ Γ |- t ≅ u : A ] ->
+        [ Γ |- tApp f t ≅ tApp g u : B{0 := t} ]
+  }.
+
+  Class OneRedTypeProp :=
+  {
+    oredty_whnf {Γ N A} :
+      whnf Γ N -> [Γ |- N ⇒ A] -> False ;
+    oredty_det {Γ T U V} :
+      [Γ |- T ⇒ U] -> [Γ |- T ⇒ V] ->
+      U = V ;
+    oredty_term {Γ A B} :
+    [Γ |- A ⇒ B : U] -> [Γ |- A ⇒ B]
+  }.
+
+  Class OneRedTermProp :=
+  {
+    oredtm_whnf {Γ n u A} :
+      whnf Γ n -> [Γ |- n ⇒ u : A] -> False ;
+    oredtm_det {Γ A B t u v} :
+      [Γ |- t ⇒ u : A] -> [Γ |- t ⇒ v : B] ->
+      u = v ;
+    oredtm_beta {Γ na A B t u} :
+      [ Γ |- A ] ->
+      [ Γ ,, vass na A |- t : B ] ->
+      [ Γ |- u : A ] ->
+      [ Γ |- tApp (tLambda na A t) u ≅ t{0 := u} : B{0 := u} ] ;
+    oredtm_app {Γ na A B f f' t} :
+      [ Γ |- f ⇒ f' : tProd na A B ] ->
+      [ Γ |- t : A ] ->
+      [ Γ |- tApp f t ⇒ tApp f' t : B{0 := t} ];
+    oredtm_conv {Γ t u A A'} : 
+      [Γ |- t ⇒ u : A] ->
+      [Γ |- A ≅ A'] ->
+      [Γ |- t ⇒ u : A']
+  }.
+
+End GenericTyping.
+
+
+Class GenericTypingProp `(GenericTypingData) :=
+{
+  wfc_prop :> WfContextProp ;
+  wfty_prop :> WfTypeProp ;
+  typ_prop :> TypingProp ;
+  convty_prop :> ConvTypeProp ;
+  convtm_prop :> ConvTermProp ;
+  convne_prop :> ConvNeuProp ;
+  redty_prop :> OneRedTypeProp ;
+  redtm_prop :> OneRedTermProp ;
+}.
+
+#[export] Hint Resolve wfc_nil wfc_cons wft_U wft_prod ty_var ty_prod ty_lam ty_app convty_wk convty_uni convty_prod convtm_wk convtm_prod convtm_eta convneu_wk convneu_var convneu_app oredty_term oredtm_beta oredtm_app | 2 : gen_typing.
+#[export] Hint Resolve wft_term ty_conv convty_term convtm_conv convneu_conv oredtm_conv | 4 : gen_typing.
+
+Section GenericConsequences.
+  Context `{tyP : GenericTypingProp}.
+  Open Scope untagged_scope.
+
+  Definition mredtm_conv {Γ t u A B} :
+      [Γ |- t ⇒* u : A] ->
+      [Γ |- A ≅ B] ->
+      [Γ |- t ⇒* u : B].
+  Proof.
+    induction 1.
+    all: econstructor ; gen_typing.
+  Qed.
+
+  Definition wfredtm_conv {Γ} {t u A B} :
+      [Γ |- t :⇒*: u : A] ->
+      [Γ |- A ≅ B] ->
+      [Γ |- t :⇒*: u : B].
+  Proof.
+    intros [? ? red] conv.
+    constructor.
+    1-2: gen_typing.
+    clear - tyP red conv.
+    induction red ; gen_typing.
+  Qed.
+
+  Lemma mredtm_whnf Γ t u A : [Γ |- t ⇒* u : A] -> whnf Γ t -> t = u.
+  Proof.
+    intros [] ?.
+    1: reflexivity.
+    exfalso.
+    eauto using oredtm_whnf.
+  Qed.
+
+  Corollary mredty_whnf Γ A B : [Γ |- A ⇒* B] -> whnf Γ A -> A = B.
+  Proof.
+    intros [] ?.
+    1: reflexivity.
+    exfalso.
+    now eauto using oredty_whnf.
+  Qed.
+
+  Lemma whredtm_mredtm_det Γ t u u' A A' :
+  [Γ |- t ↘ u : A] -> [Γ |- t ⇒* u' : A'] ->
+  [Γ |- u' ↘ u : A].
+  Proof.
+    intros [red whnf] red'.
+    induction red in whnf, A', u', red' |- *.
+    - constructor ; tea.
+      eapply mredtm_whnf in red' as -> ; tea.
+      now econstructor.
+    - destruct red' as [? | ? ? ? ? o'].
+      + econstructor.
+        2: gen_typing.
+        now econstructor.
+      + unshelve epose proof (oredtm_det o o') as <-.
+        now eapply IHred.
+  Qed.
+
+  Corollary whredtm_det Γ t u u' A A' :
+    [Γ |- t ↘ u : A] -> [Γ |- t ↘ u' : A'] ->
+    u = u'.
+  Proof.
+    intros red [].
+    eapply whredtm_mredtm_det in red as [] ; tea.
+    symmetry.
+    now eapply mredtm_whnf.
+  Qed.
+
+  Lemma whredty_mredty_det Γ A B B' :
+    [Γ |- A ↘ B] -> [Γ |- A ⇒* B'] ->
+    [Γ |- B' ↘ B].
+  Proof.
+    intros [red whnf] red'.
+    induction red in whnf, B', red' |- *.
+    - eapply mredty_whnf in red' as -> ; tea.
+      gen_typing.
+    - destruct red' as [| ? ? ? red'].
+      1: gen_typing.
+      now epose proof (oredty_det o red') as <-.
+  Qed.
+
+  Corollary nred_det_ty Γ A B B' :
+    [Γ |- A ↘ B] -> [Γ |- A ↘ B'] ->
+    B = B'.
+  Proof.
+    intros red [].
+    eapply whredty_mredty_det in red as [] ; tea.
+    symmetry.
+    now eapply mredty_whnf.
+  Qed.
+
+End GenericConsequences.
