theories/Notations.v
@@ -1,15 +1,114 @@
-(** Declarative Typing *)
+From MetaCoq.PCUIC Require Import PCUICAst PCUICAstUtils PCUICSigmaCalculus.
+
+(* We have two families of definitions: the declarative ones (tagged de), and the algorithmic ones (tagged al) *)
+(* All notations come in two versions: the tagged and the untagged one. One or the other can be used by variating the scope, in order to use tags only when needed to disambiguate between different instances of typing. *)
+
+Variant tag := | de | al.
+
+Declare Scope tagged_scope.
+Delimit Scope tagged_scope with tagged.
+Declare Scope untagged_scope.
+Delimit Scope untagged_scope with untagged.
+
+(** Typing *)
+Class WfContext (ta : tag) := wf_context : context -> Type.
+Class WfType (ta : tag) := wf_type : context -> term -> Type.
+Class Typing (ta : tag) := typing : context -> term -> term -> Type.
+Class ConvType (ta : tag) := conv_type : context -> term -> term -> Type.
+Class ConvTerm (ta : tag) := conv_term : context -> term -> term -> term -> Type.
+Class ConvNeu (ta : tag) := conv_neu : context -> term -> term -> term -> Type.
+
 (* The context Γ is well-formed *)
-Reserved Notation "[   |- Γ ]" (at level 0, Γ at level 50).
+Notation "[ |- Γ ]" := (wf_context Γ)
+  (at level 0, Γ at level 50) : untagged_scope.
+Notation "[ |-[ ta  ] Γ ]" := (wf_context (ta := ta) Γ)
+  (at level 0, ta, Γ at level 50) : tagged_scope.
 (* The type A is well-formed in Γ *)
-Reserved Notation "[ Γ |- A ]" (at level 0, Γ, A at level 50).
+Notation "[ Γ |- A ]" := (wf_type Γ A)
+  (at level 0, Γ, A at level 50) : untagged_scope.
+Notation "[ Γ |-[ ta  ] A ]" := (wf_type (ta := ta) Γ A)
+  (at level 0, ta, Γ, A at level 50) : tagged_scope.
 (* The term t has type A in Γ *)
-Reserved Notation "[ Γ |- t : A ]" (at level 0, Γ, t, A at level 50).
-(* Types A and B are (declaratively) convertible in Γ *)
-Reserved Notation "[ Γ |- A ≅ B ]" (at level 0, Γ, A, B at level 50).
-(* Terms t and t' are (declaratively) convertible in Γ *)
-Reserved Notation "[ Γ |- t ≅ t' : A ]" (at level 0, Γ, t, t', A at level 50).
+Notation "[ Γ |- t : A ]" := (typing Γ t A)
+  (at level 0, Γ, t, A at level 50) : untagged_scope.
+Notation "[ Γ |-[ ta  ] t : A ]" :=
+  (typing (ta := ta) Γ t A) (at level 0, ta, Γ, t, A at level 50) : tagged_scope.
+(* Types A and B are convertible in Γ *)
+Notation "[ Γ |- A ≅ B ]" := (conv_type Γ A B)
+  (at level 0, Γ, A, B at level 50) : untagged_scope.
+Notation "[ Γ |-[ ta  ] A ≅ B ]" := (conv_type (ta := ta) Γ A B)
+  (at level 0, ta, Γ, A, B at level 50) : tagged_scope.
+(* Terms t and t' are convertible in Γ *)
+Notation "[ Γ |- t ≅ t' : A ]" := (conv_term Γ t t' A)
+  (at level 0, Γ, t, t', A at level 50) : untagged_scope.
+Notation "[ Γ |-[ ta  ] t ≅ t' : A ]" := (conv_term (ta := ta) Γ t t' A)
+  (at level 0, ta, Γ, t, t', A at level 50) : tagged_scope.
+(* Neutral n and n' are convertible in Γ *)
+Notation "[ Γ |- n ~ n' : A ]" := (conv_neu Γ n n' A)
+  (at level 0, Γ, n, n', A at level 50) : untagged_scope. 
+Notation "[ Γ |-[ ta  ] n ~ n' : A ]" := (conv_neu (ta := ta) Γ n n' A)
+  (at level 0, ta, Γ, n, n', A at level 50) : tagged_scope.
+
+(** Reductions *)
+Class OneRedType (ta : tag) := one_red_ty : context -> term -> term -> Type.
+Class OneRedTerm (ta : tag) := one_red_tm : context -> term -> term -> term -> Type.
+(* Class MultiRedType := multi_red_ty : context -> term -> term -> Type.
+Class MultiRedTerm := multi_red_tm : context -> term -> term -> term -> Type.
+Class WhNormType := wh_norm_ty : context -> term -> term -> Type.
+Class WhNormTerm := wh_norm_tm : context -> term -> term ->term -> Type. *)
+
 (* Type A one-step weak-head reduces to type B in Γ *)
+Notation "[ Γ |- A ⇒ B ]" := (one_red_ty Γ A B)
+  (at level 0, Γ, A, B at level 50) : untagged_scope.
+Notation "[ Γ |-[ ta  ] A ⇒ B ]" := (one_red_ty (ta := ta) Γ A B)
+  (at level 0, ta, Γ, A, B at level 50) : tagged_scope.
+(* Term t one-step weak-head reduces to term u at type A in Γ *)
+Notation "[ Γ |- t ⇒ u : A ]" := (one_red_tm Γ t u A)
+  (at level 0, Γ, t, u, A at level 50) : untagged_scope.
+Notation "[ Γ |-[ ta  ] t ⇒ u : A ]" := (one_red_tm (ta := ta) Γ t u A)
+  (at level 0, ta, Γ, t, u, A at level 50) : untagged_scope.
+(* Type A multi-step weak-head reduces to type B in Γ *)
+Reserved Notation "[ Γ |- A ⇒* B ]" (at level 0, Γ, A, B at level 50).
+Reserved Notation "[ Γ |-[ ta  ] A ⇒* B ]" (at level 0, ta, Γ, A, B at level 50).
+(* Term t multi-step weak-head reduces to term t' at type A in Γ *)
+Reserved Notation "[ Γ |- t ⇒* t' : A ]" (at level 0, Γ, t, t', A at level 50).
+Reserved Notation "[ Γ |-[ ta  ] t ⇒* t' : A ]" (at level 0, ta, Γ, t, t', A at level 50).
+(* Type A weak-head normalizes to B in Γ, ie it multi-step reduces to the weak-head normal form B*)
+Reserved Notation "[ Γ |- A ↘ B ]" (at level 0, Γ, A, B at level 50).
+Reserved Notation "[ Γ |-[ ta  ] A ↘ B ]" (at level 0, ta, Γ, A, B at level 50).
+(* Term t weak-head normalizes to u at type A in Γ *)
+Reserved Notation "[ Γ |- t ↘ u : A ]" (at level 0, Γ, t, u, A at level 50).
+Reserved Notation "[ Γ |-[ ta  ] t ↘ u : A ]" (at level 0, ta, Γ, t, u, A at level 50).
+
+(** Substitutions *)
+
+Class WfSubst (ta : tag) := wf_subst : context -> substitution -> context -> Type.
+Class ConvSubst (ta : tag) := conv_subst : context -> substitution -> substitution -> context -> Type.
+
+(* Substitution σ is of type Δ in context Γ*)
+Notation "[ Γ '|-s' σ : Δ ]" := (wf_subst Γ σ Δ)
+  (at level 0, Γ, σ, Δ at level 50) : untagged_scope.
+Notation "[ Γ '|-'[ ta  ']s' σ : Δ ]" := (wf_subst (ta := ta) Γ σ Δ)
+  (at level 0, ta, Γ, σ, Δ at level 50) : tagged_scope.
+(* Substitutions σ and τ are convertible at types Δ in context Γ *)
+Notation "[ Γ '|-s' σ ≅ τ : Δ ]" := (conv_subst Γ σ τ Δ)
+  (at level 0, Γ, σ, τ, Δ at level 50) : untagged_scope.
+Notation "[ Γ '|-[ ta ']s' σ ≅ τ : Δ ]" := (conv_subst (ta := ta) Γ σ τ Δ)
+  (at level 0, ta, Γ, σ, τ, Δ at level 50) : tagged_scope.
+
+(** Extra typing conditions *)
+(* Types A and B are well-formed and convertible in Γ *)
+Reserved Notation "[ Γ |- A :≅: B ]" (at level 0, Γ, A, B at level 50).
+Reserved Notation "[ Γ |-[ ta  ] A :≅: B ]" (at level 0, ta, Γ, A, B at level 50).
+(* Terms t and u are well-typed and convertible at type A in Γ *)
+Reserved Notation "[ Γ |- t :≅: u : A ]" (at level 0, Γ, t, u, A at level 50).
+Reserved Notation "[ Γ |-[ ta  ] t :≅: u : A ]" (at level 0, ta, Γ, t, u, A at level 50).
+(* Type A and B are well-formed and A weak-head reduces to B in Γ *)
+Reserved Notation "[ Γ |- A :⇒*: B ]" (at level 0, Γ, A, B at level 50).
+Reserved Notation "[ Γ |-[ ta  ] A :⇒*: B ]" (at level 0, ta, Γ, A, B at level 50).
+(* Terms t and u have type A in Γ and t weak-head reduces to u *)
+Reserved Notation "[ Γ |- t :⇒*: u : A ]" (at level 0, Γ, t, u, A at level 50).
+Reserved Notation "[ Γ |-[ ta  ] t :⇒*: u : A ]" (at level 0, ta, Γ, t, u, A at level 50).
 
 (** Weakenings *)
 (* Well-formed weakening *)
@@ -17,41 +116,8 @@ Reserved Notation "Γ ≤ Δ" (at level 40).
 (* Composition of weakenings *)
 Reserved Notation "ρ ∘w ρ'" (at level 50).
 
-(** Substitutions *)
-(* Substitution σ is of type Δ in context Γ*)
-Reserved Notation "[ Γ '|-s' σ : Δ ]" (at level 0, Γ, σ, Δ at level 50).
-(* Substitutions σ and τ are convertible at types Δ in context Γ *)
-Reserved Notation "[ Γ '|-s' σ ≅ τ : Δ ]" (at level 0, Γ, σ, τ, Δ at level 50).
-
-(** Reductions *)
-Reserved Notation "[ Γ |- A ⇒ B ]" (at level 0, Γ, A, B at level 50).
-(* Term t one-step weak-head reduces to term u at type A in Γ *)
-Reserved Notation "[ Γ |- t ⇒ u : A ]" (at level 0, Γ, t, u, A at level 50).
-(* Type A multi-step weak-head reduces to type B in Γ *)
-Reserved Notation "[ Γ |- A ⇒* B ]" (at level 0, Γ, A, B at level 50).
-(* Term t multi-step weak-head reduces to term t' at type A in Γ *)
-Reserved Notation "[ Γ |- t ⇒* t' : A ]" (at level 0, Γ, t, t', A at level 50).
-(* Type A weak-head reduces in at least one step to type B in Γ *)
-Reserved Notation "[ Γ |- A ⇒⁺ B ]" (at level 0, Γ, A, B at level 50).
-(* Term t weak-head reduces in at least one step to term u at type A in Γ *)
-Reserved Notation "[ Γ |- t ⇒⁺ u : A ]" (at level 0, Γ, t, u, A at level 50).
-(* Type A weak-head normalizes to B in Γ, ie it multi-step reduces to the weak-head normal form B*)
-Reserved Notation "[ Γ |- A ↘ B ]" (at level 0, Γ, A, B at level 50).
-(* Term t weak-head normalizes to u at type A in Γ *)
-Reserved Notation "[ Γ |- t ↘ u : A ]" (at level 0, Γ, t, u, A at level 50).
-(* Types A and B are well-formed and convertible in Γ *)
-
-(** Extra typing conditions *)
-Reserved Notation "[ Γ |- A :≅: B ]" (at level 0, Γ, A, B at level 50).
-(* Terms t and u are well-typed and convertible at type A in Γ *)
-Reserved Notation "[ Γ |- t :≅: u : A ]" (at level 0, Γ, t, u, A at level 50).
-(* Type A and B are well-formed and A weak-head reduces to B in Γ *)
-Reserved Notation "[ Γ |- A :⇒*: B ]" (at level 0, Γ, A, B at level 50).
-(* Terms t and u have type A in Γ and t weak-head reduces to u *)
-Reserved Notation "[ Γ |- t :⇒*: u : A ]" (at level 0, Γ, t, u, A at level 50).
 
 (** Logical relation *)
-
 (* The universe is reducible in Γ, according to the kit K *)
 Reserved Notation "[ K | Γ ||-U ]" (at level 0, K, Γ at level 50).
 (* The type A is reducible as a product type in Γ according to the kit K *)
